verification/theories/page_table/page_table.v
@@ -1,10 +1,255 @@
 From refinedrust Require Import typing.
 From ace.theories.page Require Import page_extra.
+From stdpp Require Import bitvector.
+
+(* Based on Release riscv-isa-release-7b8ddc9-2024-05-07 *)
+
+(** Basic defs *)
+Definition bv_to_bit {n : N} (m : nat) (bv : bv n) : bool :=
+  bv_to_bits bv !!! m.
+
+Definition bit_to_bv (b : bool) : bv 1 :=
+  bool_to_bv 1 b.
 
 (** * Architectural ground-truth *)
 (* TODO: have file for translated sail specs and then link up with this *)
 
-Inductive pte_flags_bits : Type :=
+(** ** Paging system *)
+(* Currently we only include the supported paging systems *)
+Inductive paging_system :=
+  | Sv57.
+
+Global Instance paging_system_eqdec : EqDecision paging_system.
+Proof. unfold EqDecision, Decision. intros. destruct x, y; decide equality. Qed.
+
+(** The virtual address length *)
+Definition paging_system_virtual_address_length (sys : paging_system) : N :=
+  match sys with
+  | Sv57 => 57
+  end.
+
+(** The physical address length *)
+Definition physical_address_length : N := 56.
+
+(** ** PTE Flags *)
+Record pte_flags : Type := mk_pte_flags {
+  (* 0 *)
+  PTEValid : bool;
+  (* 1 *)
+  PTERead : bool;
+  (* 2 *)
+  PTEWrite : bool;
+  (* 3 *)
+  PTEExecute : bool;
+  (* 4 *)
+  PTEUser : bool;
+  (* 5 *)
+  PTEGlobal : bool;
+  (* 6 *)
+  PTEAccessed : bool;
+  (* 7 *)
+  PTEDirty : bool;
+}.
+
+Definition pte_flags_invalid : pte_flags :=
+  mk_pte_flags false false false false false false false false.
+
+(* Decode PTE flags *)
+Definition pte_decode_flags (pte : bv 7) : pte_flags :=
+  mk_pte_flags
+    (bv_to_bit 0 pte)
+    (bv_to_bit 1 pte)
+    (bv_to_bit 2 pte)
+    (bv_to_bit 3 pte)
+    (bv_to_bit 4 pte)
+    (bv_to_bit 5 pte)
+    (bv_to_bit 6 pte)
+    (bv_to_bit 7 pte)
+.
+
+(* Encode PTE flags *)
+Definition pte_encode_flags (flags : pte_flags) : bv 8 :=
+  bv_concat 8 (bit_to_bv flags.(PTEDirty))
+    $ bv_concat 7 (bit_to_bv flags.(PTEAccessed))
+    $ bv_concat 6 (bit_to_bv flags.(PTEGlobal))
+    $ bv_concat 5 (bit_to_bv flags.(PTEUser))
+    $ bv_concat 4 (bit_to_bv flags.(PTEExecute))
+    $ bv_concat 3 (bit_to_bv flags.(PTEWrite))
+    $ bv_concat 2 (bit_to_bv flags.(PTERead))
+    (bit_to_bv flags.(PTEValid))
+.
+
+(* Check if PTE is a pointer to next level (non-leaf) *)
+Definition pte_is_ptr (flags : pte_flags) : bool :=
+  (negb flags.(PTERead)) && (negb flags.(PTEWrite)) && (negb flags.(PTEExecute))
+.
+
+(* Check if PTE is valid *)
+Definition pte_is_invalid (flags : pte_flags) : bool :=
+  (negb flags.(PTEValid)) 
+  (* TODO: security monitor does not have to check for it *)
+  || (flags.(PTEWrite) && negb flags.(PTERead))
+.
+
+
+(** ** PTE *)
+
+(** Get the bits describing the flags *)
+Definition pte_get_flags_bits (pte : bv 64) : bv 8 :=
+  bv_extract 0 8 pte.
+
+(** Get the bits describing the rsw *)
+Definition pte_get_rsw_bits (pte : bv 64) : bv 2 :=
+  bv_extract 8 2 pte.
+
+(** Get the bits describing the ppn *)
+Definition pte_ppn_length : N := 44.
+Definition pte_get_ppn_bits (pte : bv 64) : bv pte_ppn_length :=
+  bv_extract 10 pte_ppn_length pte.
+
+(** Get the bits for the pbmt extension *)
+Definition pte_get_pbmt_bits (pte : bv 64) : bv 2 :=
+  bv_extract (pte_ppn_length + 10) 2 pte.
+
+(** Get the bits for the napot extension *)
+Definition pte_get_napot_bits (pte : bv 64) : bv 1 :=
+  bv_extract (pte_ppn_length + 10 + 2) 1 pte.
+
+
+
+(** Encode a physical address for a PPN entry *)
+Definition encode_physical_address_to_ppn (addr : Z) : bv pte_ppn_length :=
+  (* Ignore the 12 lowest bits. We have to wrap around for addresses which exceed physical size, as the higher bits are required to replicate the 56th bit. *)
+  bv_extract 12 pte_ppn_length (Z_to_bv physical_address_length addr)
+.
+
+(** A valid physical address should fit into 64 bits. The highest 8 bits should replicate the 56th bit. *)
+Definition is_valid_physical_address (addr : Z) :=
+  ∃ bv_addr, 
+    Z_to_bv_checked 64 addr = Some bv_addr ∧
+    Forall (λ x, bv_to_bit (N.to_nat physical_address_length) bv_addr = x) (drop (N.to_nat physical_address_length) (bv_to_bits bv_addr)).
+
+(** Encode a page table entry *)
+Definition encode_pte
+  (phys_addr : Z)
+  (flags : pte_flags) : bv 64 :=
+  (* The leading bits up to the PPN are zero, including pbmt and napot bits *)
+  bv_concat 64 (encode_physical_address_to_ppn phys_addr) (* PPN *)
+    $ bv_concat 10 (bv_0 2) (* RSW *)
+    $ pte_encode_flags flags (* flags *)
+.
+
+(* 
+  ∀ guest_physical_address, 
+    memory_isolation_translate (some_hw_config) serialized_page_table guest_phyiscal_address = Some real_address →
+   real_address belongs to this VM
+
+
+   (* TODO: does it suffice to prove a weaker property? *)
+
+   is_byte_level_logical_representation logical physical →
+
+   we also need to require that the hardware actually does an exception if the translation fails.
+
+
+
+   What is the right way to formalize this?
+   Probably we need a logical version and a physical version.
+
+   The physical version is used by the semantics, and it requires access to the whole state in order to follow pointers
+   The logical version should be used in our spec, and correspond to the physical version, in that it translates to the same things.
+
+
+ *)
+
+    
+
+(* Notes:
+  all of RWX are zero => pointer to next level
+  otherwise a leaf
+
+  W implies R
+
+  SUM bit determines whether supervisor can access user mode pages
+
+  G exists in all address spaces. 
+
+  leaves contain A D U; for non-leafs, they have to be cleared
+
+
+  How does the shape of the page table relate between the one for guest translation and supervisor translation? 
+   Sv57x4 is for guest physical to supervisor physical
+  So does the hypervisor also go through this scheme, or is that using Sv57?
+   => It's using Sv57. But the hypervisor page table is not managed by the security monitor.
+    It's setup by the hypervisor boot process.
+   The security monitor only cares about correctly backing up and restoring the satp config.
+
+
+  Steps for formalization:
+   - convert bit sequence to integer
+   - stuff to concatenate bit sequences
+
+ *)
+
+Definition translate_address (pt_addr : Z) (σ : state) (addr : Z) : option Z :=
+  None
+. 
+
+
+(** * Logical representation *)
+(** Configuration of the page table entry *)
+Record page_table_config : Type := mk_ptc {
+  pt_accessible_to_user : bool;
+  pt_was_accessed : bool;
+  pt_is_global_mapping : bool;
+  pt_is_dirty : bool;
+}.
+Global Instance page_table_config_inh : Inhabited page_table_config := populate (mk_ptc false false false false).
+
+
+(** Permissions for this page table entry *)
+Record page_table_permission : Type := mk_ptp {
+  ptp_can_read : bool;
+  ptp_can_write : bool;
+  ptp_can_execute : bool;
+}.
+Global Instance page_table_permission_inh : Inhabited page_table_permission := populate (mk_ptp false false false).
+
+Definition pt_permission_pointer : page_table_permission :=
+  mk_ptp false false false.
+
+(** Encode page table flags *)
+Definition to_pte_flags (valid : bool) (ptc : page_table_config) (ptp : page_table_permission) : pte_flags := {|
+  PTEValid := valid;
+  PTERead := ptp.(ptp_can_read);
+  PTEWrite := ptp.(ptp_can_write);
+  PTEExecute := ptp.(ptp_can_execute);
+  PTEUser := ptc.(pt_accessible_to_user);
+  PTEGlobal := ptc.(pt_is_global_mapping);
+  PTEAccessed := ptc.(pt_was_accessed);
+  PTEDirty := ptc.(pt_is_dirty);
+|}.
+
+(** 
+  How do we decode things? 
+  Should we take an integer or another type? 
+   Idea: define a bitvector type that at least requires that it's in the given bitwidth. 
+   But I guess this is already given by the integer type itself.
+   I could represent it as a list of bits, instead. 
+   But encoding/decoding should anyways be reversible. So it wouldn't change much.
+    decode (encode bits) = Some bits
+    decode i = Some bits → encode bits = i
+
+  I guess the main advantage is that it's easier to do stuff with masking etc. 
+   
+  Especially with or-ing stuff. 
+   that will be difficult to do otherwise. 
+
+*)
+(*Definition *)
+
+(** The valid PTE flag bits. *)
+Inductive pte_flags_bits :=
   | PTValid
   | PTRead
   | PTWrite
@@ -14,38 +259,14 @@ Inductive pte_flags_bits : Type :=
   | PTAccessed
   | PTDirty
 .
-Definition pte_flags_bits_bits_position (b : pte_flags_bits) :=
-  match b with
-  | PTValid => 0
-  | PTRead => 1
-  | PTWrite => 2
-  | PTExecute => 3
-  | PTUser => 4
-  | PTGlobal => 5
-  | PTAccessed => 6
-  | PTDirty => 7
-  end.
 
-(** * Logical representation *)
-Record page_table_config : Type := {
-  pt_accessible_to_user : bool;
-  pt_was_accessed : bool;
-  pt_is_global_mapping : bool;
-  pt_is_dirty : bool;
-}.
+(*Definition pte_flags_bits_mask *)
 
-Record page_table_permission : Type := {
-  ptp_can_read : bool;
-  ptp_can_write : bool;
-  ptp_can_execute : bool;
-}.
 
 Record shared_page : Type := {
-  (* TODO *)
+  shared_page_hv_address : Z;
+  shared_page_sz : page_size;
 }.
-
-Inductive paging_system :=
-  | Sv57x4.
 
 Inductive page_table_level :=
   | PTLevel5
@@ -54,7 +275,16 @@ Inductive page_table_level :=
   | PTLevel2
   | PTLevel1.
 
+Global Instance page_table_level_eqdec : EqDecision page_table_level.
+Proof. solve_decision. Qed.
 
+Definition paging_system_highest_level (system : paging_system) : page_table_level :=
+  match system with
+  | Sv57x4 => PTLevel5
+  end.
+
+Definition number_of_page_table_entries (system : paging_system) (level : page_table_level) : nat :=
+  if decide (level = paging_system_highest_level system) then 2048%nat else 512%nat.
 
 (* Can we avoid mutual inductives? *)
 Inductive page_table_entry : Type :=
@@ -77,23 +307,34 @@ Inductive page_table_entry : Type :=
 with page_table_tree :=
   | PageTableTree
       (system : paging_system)
+      (serialized_addr : Z)
       (entries : list page_table_entry)
       (level : page_table_level)
 .
 
-Definition pg_get_system (pg : page_table_tree) : paging_system :=
+Definition pt_get_system (pt : page_table_tree) : paging_system :=
   match pt with
-  | PageTableTree system _ _ => system
+  | PageTableTree system _ _ _ => system
   end.
 
 Definition pt_get_level (pt : page_table_tree) : page_table_level :=
   match pt with
-  | PageTableTree _ level => level
+  | PageTableTree _ _ _ level => level
   end.
 
 Definition pt_get_entries (pt : page_table_tree) : list page_table_entry :=
   match pt with
-  | PageTableTree entries _ => entries
+  | PageTableTree _ _ entries _ => entries
+  end.
+
+Definition pt_get_serialized_addr (pt : page_table_tree) : Z :=
+  match pt with
+  | PageTableTree _ loc _ _ => loc
+  end.
+
+Definition pt_number_of_entries (pt : page_table_tree) : nat :=
+  match pt with
+  | PageTableTree system _ _ level => number_of_page_table_entries system level
   end.
 
 (*Fixpoint page_table_levels_decreasing (p : page_table_tree) :=*)
@@ -105,47 +346,66 @@ Definition pt_get_entries (pt : page_table_tree) : list page_table_entry :=
   (*match pt with*)
   (*| PointerToNextPageTable next conf =>*)
 
-Definition paging_system_highest_level (system : paging_system) : page_table_level :=
-  match system with
-  | Sv57x4 => PTLevel5
-  end.
-
-Definition number_of_page_table_entries (system : paging_system) (level : page_table_level) : nat :=
-  if decide (level = paging_system_highest_level system) then 2048 else 512.
-
-Definition pt_number_of_entries (pt : page_table_tree) : nat :=
+Fixpoint page_table_tree_has_system (system : paging_system) (pt : page_table_tree) :=
   match pt with
-  | PageTableTree system level _ => number_of_page_table_entries system level
+  | PageTableTree system' _ entries _ =>
+      system = system' ∧
+      Forall_cb (page_table_entry_has_system system) entries
+  end
+with page_table_entry_has_system (system : paging_system) (pte : page_table_entry) :=
+  match pte with
+  | PointerToNextPageTable pt _ =>
+      page_table_tree_has_system system pt
+  | _ => 
+      True
   end.
+
 
 (* TODO: maybe make this intrinsic using dependent type *)
-Definition page_table_wf (t : page_table_tree) :=
+Definition page_table_wf (pt : page_table_tree) :=
   (* number of page table entries is determined by the level *)
-  (match t with | PageTableTree entries level => number_of_page_table_entries level = length entries end) ∧
+  number_of_page_table_entries (pt_get_system pt) (pt_get_level pt) = length (pt_get_entries pt) ∧
   (* ensure that levels are decreasing *)
   (* TODO *)
   (* ensure that the system is the same across the whole page table *)
-  (* TODO *)
-  True
+  page_table_tree_has_system (pt_get_system pt) pt
 .
 (* TODO: ensure everything is in confidential memory *)
 
 
-(** Encoding *)
-Definition encode_page_table_entry (pte : page_table_entry) : Z :=
-  (* TODO *)
-  0.
+Definition make_empty_page_tree (system : paging_system) (level : page_table_level) (loc : Z) := 
+  PageTableTree system loc [] level.
 
+(** Encoding *)
+Definition encode_page_table_entry_bv (pte : page_table_entry) : bv 64 :=
+  match pte with
+  | PointerToNextPageTable pt ptc =>
+      (* This is not a leaf *)
+      encode_pte (pt_get_serialized_addr pt) (to_pte_flags true ptc pt_permission_pointer)
+  | PageWithConfidentialVmData pg ptc ptp =>
+      encode_pte pg.(page_loc).2 (to_pte_flags true ptc ptp)
+  | PageSharedWithHypervisor sp ptc ptp =>
+      encode_pte sp.(shared_page_hv_address) (to_pte_flags true ptc ptp)
+  | NotValid =>
+      encode_pte 0 pte_flags_invalid
+  end
+.
+Definition encode_page_table_entry (pte : page_table_entry) : Z :=
+  bv_unsigned $ encode_page_table_entry_bv pte.
 Definition encode_page_table_entries (entries : list page_table_entry) : list Z :=
   encode_page_table_entry <$> entries
 .
 
+(** Relation that states that [pt_byte] is a valid byte-level representation of [pt_logical]'s entries. *)
 Definition is_byte_level_representation (pt_logical : page_table_tree) (pt_byte : page) :=
+  (* The physical address matches up *)
+  pt_byte.(page_loc).2 = pt_get_serialized_addr pt_logical ∧
   (* The logical representation is well-formed *)
   page_table_wf pt_logical ∧
   (* We have a 16KiB page for Level 5, and 4KiB pages otherwise *)
   (if pt_get_level pt_logical is PTLevel5 then pt_byte.(page_sz) = Size16KiB else pt_byte.(page_sz) = Size4KiB) ∧
   (* The encoding of the entries matches the physical content of the pages *)
+  (* NOTE: if the list of entries is [], this should be trivial. *)
   pt_byte.(page_val) = encode_page_table_entries (pt_get_entries pt_logical)
 .
 
@@ -153,9 +413,36 @@ Definition is_byte_level_representation (pt_logical : page_table_tree) (pt_byte 
 (** Operations modifying the page table *)
 Definition pt_set_entry (pt : page_table_tree) (index : nat) (entry : page_table_entry) : page_table_tree :=
   match pt with
-  | PageTableTree system level entries =>
-      PageTableTree system level (<[index := entry]> entries)
+  | PageTableTree system serialized_addr entries level =>
+      PageTableTree system serialized_addr (<[index := entry]> entries) level
   end.
 
-Lemma pt_set_entry_wf : 
-  pt_set
+(*Lemma pt_set_entry_wf : *)
+  (*pt_set*)
+
+(** ** Using a page table *)
+(** Translate an address according to the logical page table representation *)
+Definition page_table_translate_address (pt : page_table_tree)  (addr : Z) : option Z :=
+  None.
+
+(** State that the page table is represented at a particular root address in memory *)
+Definition pt_represented_at (σ : state) (pt : page_table_tree) (pt_addr : Z) :=
+  (* TODO *)
+  False.
+
+(** Address translation should be consistent between the logical and physical version *)
+Lemma page_table_translate_address_consistent_1 (pt : page_table_tree) addr pt_addr σ translated_addr : 
+  pt_represented_at σ pt pt_addr →
+  page_table_translate_address pt addr = Some translated_addr →
+  translate_address pt_addr σ addr = Some translated_addr
+.
+Proof.
+Abort.
+
+Lemma page_table_translate_address_consistent_2 pt addr pt_addr σ translated_addr : 
+  pt_represented_at σ pt pt_addr →
+  translate_address pt_addr σ addr = Some translated_addr →
+  page_table_translate_address pt addr = Some translated_addr
+.
+Proof.
+Abort.
